Construction of A
Mostly decidable equality for all types

proofs/core/ADTAlt.v
@@ -1,10 +1,88 @@
 Require Import Coq.Strings.String.
 Require Import Coq.Lists.List.
+Require Import Coq.Bool.Bool.
+Import ListNotations.
+
+From mathcomp Require all_ssreflect. (*fintype finfun.*)
+
+Set Bullet Behavior "Strict Subproofs".
+
+Coercion proj_sumbool (A B: Prop) (H: {A} + {B}) : bool :=
+  if H then true else false.
+Coercion is_true : bool >-> Sortclass.
+
+(*TODO: Separate file*)
+Section Util.
+
+Inductive ForallT {A: Type} (P: A -> Type) : list A -> Type :=
+  | ForallT_nil: ForallT P nil
+  | ForallT_cons: forall {x: A} {l: list A},
+    P x -> ForallT P l -> ForallT P (x :: l).
+
+Lemma ForallT_hd {A: Type} {P: A -> Type} {x: A} {l: list A}:
+  ForallT P (x :: l) ->
+  P x.
+Proof.
+  intros. inversion X; subst. apply X0.
+Qed.
+
+Lemma ForallT_tl {A: Type} {P: A -> Type} {x: A} {l: list A}:
+  ForallT P (x :: l) ->
+  ForallT P l.
+Proof.
+  intros. inversion X; auto.
+Qed.
+
+(*This awkward definition satisfies Coq's positivity checker
+  for nested induction, unlike the normal one*)
+  Definition map2 {A B C: Type} :=
+    fun (f: A -> B -> C) =>
+      fix map2 (l1: list A) : list B -> list C :=
+        match l1 with
+        | nil => fun l2 => nil
+        | x1 :: t1 =>
+          fun l2 =>
+          match l2 with
+          | nil => nil
+          | x2 :: t2 => f x1 x2 :: map2 t1 t2
+          end
+        end.
+
+End Util.
+
+(*TODO: move*)
+(*In many places, we need the type {x : T | in x l} and the type T is
+  decidable. We give utilities here for this type*)
+Module InType.
+
+(*First do without ssreflect, do we need?*)
+Section InTypeDef.
+Variable (T: Set). (*Set?*)
+Variable (T_dec: forall (x y: T), {x = y} + {x <> y}).
+
+Definition inb (x: T) (l: list T) : bool :=
+  fold_right (fun y acc => ((T_dec x y) || acc)) false l.
+
+Definition in_type (l: list T) : Set :=
+  { x : T | inb x l }.
+
+Definition in_type_extra (l: list T) (f: T -> Set) : Set :=
+  {t: in_type l & f (proj1_sig t)}.
+
+(*TODO: prove finite and stuff? If so, need ssreflect*)
+End InTypeDef.
+
+End InType.
+
+Import InType.
 
 Section ADT.
 
-(*The base types*)
+(*The base types (with decidable equality - we may be able to remove
+  this restriction but likely not, and it would make things MUCH worse)*)
 Variable base: Set.
+Variable base_dec: forall (x y: base), {x = y} + {x <> y}.
+
 
 (*TODO: use ssreflect? and eqType*)
 
@@ -48,7 +126,31 @@ Fixpoint ty_ind (t: ty) : P t :=
   end.
 
 End TyInd.
-(*TODO: see if we need Set/Type versions*)
+
+
+(*TODO: There has to be a better way*)
+Section TyRect.
+
+Variable (P: ty -> Type).
+Variable (Pbase: forall (b: base), P (ty_base b)).
+Variable (Pvar: forall (n: nat), P (ty_var n)).
+Variable (Papp: forall (ts: typesym) (tys: list ty),
+  ForallT P tys -> P (ty_app ts tys)).
+
+Fixpoint ty_rect (t: ty) : P t :=
+  match t with
+  | ty_base b => Pbase b
+  | ty_var n => Pvar n
+  | ty_app ts tys =>
+    Papp ts tys
+    ((fix ty_nest (l: list ty) : ForallT P l :=
+      match l with
+      | nil => ForallT_nil _
+      | x :: xs => ForallT_cons _ (ty_rect x) (ty_nest xs)
+      end) tys)
+  end.
+
+End TyRect.
 
 (*Constructors have names and a list of types*)
 Record constr : Set := {c_name: string; c_args: list ty}.
@@ -59,18 +161,244 @@ Record adt : Set := {a_name: string; a_params: nat; a_constrs: list constr}.
 (*Mutual blocks consist of a list of ADTs*)
 Record mut : Set := {m_adts: list adt}.
 
+(*TODO: is there ssreflect to do this?
+  "apply" at bottom: ex: if we have P1 -> P1 -> Q and lemma P -> Q,
+    transforms to P1 -> P2 -> P*)
+
+(*Decidable Equality*)
+Section Eq.
+Import all_ssreflect. 
+
+(*TODO: move both of these to some "Util"*)
+
+(*A version of "reflect_dec" with better computational behavior:
+  it reduces even if the "reflect" predicate is opaque*)
+Definition reflect_dec' {P} {b} (H: reflect P b): {P} + {~P} :=
+  match b as b1 return b = b1 -> _ with
+  | true => fun Heq => left (elimT H Heq)
+  | false => fun Hneq => right (elimF H Hneq)
+  end erefl.
+
+Definition typesym_eqb (t1 t2: typesym) : bool :=
+  String.eqb (ts_name t1) (ts_name t2) &&
+  Nat.eqb (ts_args t1) (ts_args t2).
+
+Ltac reflF :=
+  let C := fresh in
+  intros; apply ReflectF; intro C; inversion C; subst; contradiction.
+  
+Lemma typesym_eqb_spec (t1 t2: typesym) : reflect (t1 = t2) (typesym_eqb t1 t2).
+Proof.
+  rewrite /typesym_eqb.
+  case: (String.eqb_spec _ _); last by reflF.
+  case: (PeanoNat.Nat.eqb_spec _ _); last by reflF. 
+  (*TODO: ssreflect should be able to do this I am sure*)
+  move=> args_eq names_eq; apply ReflectT; move: args_eq names_eq.
+  by case: t1; case: t2 => n1 a1 n2 a2/=->->.
+Qed.
+
+Definition typesym_eq_dec (t1 t2: typesym) : {t1 = t2} + {t1 <> t2} :=
+  reflect_dec' (typesym_eqb_spec t1 t2).
+
+Fixpoint ty_eqb (t1 t2: ty) {struct t1} : bool :=
+  match t1, t2 with
+  | ty_base b1, ty_base b2 => base_dec b1 b2
+  | ty_var n1, ty_var n2 => Nat.eqb n1 n2
+  | ty_app ts1 tys1, ty_app ts2 tys2 =>
+    typesym_eqb ts1 ts2 &&
+    (Nat.eqb (length tys1) (length tys2)) && 
+    all id (map2 ty_eqb tys1 tys2)
+  | _, _ => false
+  end.
+
+Lemma ty_eqb_eq: forall t1 t2,
+  ty_eqb t1 t2 -> t1 = t2.
+Proof.
+  move=> t1; elim: t1 =>/=[ b1 t2 | n1 t2 | ts1 tys1 Hall t2];
+  case: t2 =>[b2 | n2 | ts2 tys2]//.
+  - by case: (base_dec b1 b2)=>//=->.
+  - by move=>/PeanoNat.Nat.eqb_spec ->.
+  - case: (typesym_eqb_spec _ _)=>//= ->.
+    case: (PeanoNat.Nat.eqb_spec _ _)=>//=.
+    move=> len_eq all_eq. f_equal.
+    move: Hall tys2 len_eq all_eq .
+    elim: tys1 =>[_ [|//] // | x tl IH Hall [//|x2 tl2] /= [] len_eq 
+      /andP[Hh Ht] ].
+    by rewrite (Forall_inv Hall _ Hh) (IH (Forall_inv_tail Hall) _ len_eq Ht).
+Qed.
+
+Lemma ty_eq_eqb: forall t1 t2,
+  t1 = t2 ->
+  ty_eqb t1 t2.
+Proof.
+  elim =>/=[b t2 <-| n t2 <- |ts tys Hall t2 <-].
+  - by case: (base_dec b b).
+  - by apply /PeanoNat.Nat.eqb_spec.
+  - case: (typesym_eqb_spec) =>//= _.
+    case: (PeanoNat.Nat.eqb_spec)=>//=_.
+    move: Hall. elim: tys => [//|x tl IH Hall/=].
+    rewrite (Forall_inv Hall) //=.
+    by apply (IH (Forall_inv_tail Hall)).
+Qed.
+
+Lemma ty_eqb_spec (t1 t2: ty):
+  reflect (t1 = t2) (ty_eqb t1 t2).
+Proof.
+  by apply iff_reflect; split; [apply ty_eq_eqb | apply ty_eqb_eq].
+Qed.
+
+Definition ty_eq_dec (t1 t2: ty): {t1 = t2} + {t1 <> t2} :=
+  reflect_dec' (ty_eqb_spec t1 t2).
+
+(*Equality on lists*)
+Fixpoint list_eqb {A: Type} (eq_dec: forall (x y: A), {x = y} + {x <> y})
+(l1 l2: list A) : bool :=
+  match l1, l2 with
+  | x1 :: t1, x2 :: t2 => eq_dec x1 x2 && list_eqb eq_dec t1 t2
+  | nil, nil => true
+  | _, _ => false
+  end.
+
+Lemma list_eqb_spec {A: Type} (eq_dec: forall (x y: A), {x = y} + {x <> y})
+(l1 l2: list A) : reflect (l1 = l2) (list_eqb eq_dec l1 l2).
+Proof.
+  move: l2. elim: l1 => [[/=|/=]|x1 t1 IH [/=|x2 t2/=]]; try by reflF.
+  - by apply ReflectT.
+  - case: (eq_dec x1 x2)=>//=[->|]; last by reflF.
+    by case: (IH t2)=>[->|]; [apply ReflectT | reflF].
+Qed.
+
+Definition list_eq_dec {A: Type} (eq_dec: forall (x y: A), {x = y} + {x <> y})
+(l1 l2: list A) : {l1 = l2} + {l1 <> l2} := reflect_dec' (list_eqb_spec eq_dec l1 l2).
+
+(*The others are much easier*)
+Definition constr_eqb (c1 c2: constr) : bool :=
+  String.eqb (c_name c1) (c_name c2) &&
+  list_eqb ty_eq_dec (c_args c1) (c_args c2).
+
+Lemma constr_eqb_spec (c1 c2: constr) : reflect (c1 = c2) (constr_eqb c1 c2).
+Proof.
+  case: c1; case: c2 => n1 a1 n2 a2; rewrite /constr_eqb/=.
+  case: String.eqb_spec=>//=[->|]; last by reflF.
+  case: list_eqb_spec=>[->|]; last by reflF.
+  by apply ReflectT.
+Qed.
+
+Definition constr_eq_dec (c1 c2: constr): {c1 = c2} + {c1 <> c2} :=
+  reflect_dec' (constr_eqb_spec c1 c2).
+
+Definition adt_eqb (a1 a2: adt) : bool :=
+  String.eqb (a_name a1) (a_name a2) &&
+  Nat.eqb (a_params a1) (a_params a2) &&
+  list_eqb constr_eq_dec (a_constrs a1) (a_constrs a2).
+
+Lemma adt_eqb_spec (a1 a2: adt) : reflect (a1 = a2) (adt_eqb a1 a2).
+Proof.
+  case: a1; case: a2 => n1 p1 c1 n2 p2 c2; rewrite /adt_eqb/=.
+  case: String.eqb_spec=>//=[->|]; last by reflF.
+  case: PeanoNat.Nat.eqb_spec=>//=[->|]; last by reflF.
+  case: list_eqb_spec=>[->|]; last by reflF.
+  by apply ReflectT.
+Qed.
+
+Definition adt_eq_dec (a1 a2: adt): {a1 = a2} + {a1 <> a2} :=
+  reflect_dec' (adt_eqb_spec a1 a2).
+
+Definition mut_eqb (m1 m2: mut) : bool :=
+  list_eqb adt_eq_dec (m_adts m1) (m_adts m2).
+
+Lemma mut_eqb_spec (m1 m2: mut) : reflect (m1 = m2) (mut_eqb m1 m2).
+Proof.
+  rewrite /mut_eqb. case: m1; case: m2 => a1 a2/=.
+  case: list_eqb_spec=>[->|]; last by reflF.
+  by apply ReflectT.
+Qed.
+
+End Eq.
+
+
 (*Basic definitions for W-types*)
 
 Section W.
 (*I is the index in the mutual block.
+  P gives the information for (uniform) polymorphism
   A is the non-recursive data for each constructor
   B tells the number of recursive arguments for each constructor*)
 Variable (I: Set).
-Variable (A: I -> Set).
-Variable (B: forall (i: I) (j: I), A i -> Set).
+Variable (P: Set).
+Variable (A: P -> I -> Set).
+Variable (B: forall (p: P) (i: I) (j: I), A p i -> Set).
+(*TODO: see about argument order*)
 
 Inductive W : I -> Set :=
-  | mkW : forall (i: I) (a: A i) (f: forall j, B i j a -> W j), W i.
+  | mkW : forall (p: P) (i: I) (a: A p i) (f: forall j, B p i j a -> W j), W i.
 
 End W.
 
+(*TODO: move*)
+Inductive empty := .
+
+Section Encode.
+
+(*All encodings for previously-declared (or abstract) type symbols
+  are given by a function typs.
+  This is allows to return anything when the length of the list is wrong*)
+(*TODO: Type?*)
+Variable (typs: typesym -> list Set -> Set).
+(*The user also specifies how base types (e.g. unit, bool, etc) are
+  interpreted*)
+Variable (bases: base -> Set).
+
+(*We encode a particular mutual type:*)
+Variable (m: mut).
+
+(*A (non-recursive) type is interpreted according to these functions.
+  Type variables are defined by a function to be given later*)
+Fixpoint ty_to_set (vars: list Set) (t: ty) : Set :=
+  match t with
+  | ty_base b => bases b
+  | ty_var v => nth v vars empty
+  | ty_app ts tys => typs ts (map (ty_to_set vars) tys)
+  end.
+
+(*We now define the type A (build_base):*)
+Section ADef.
+
+(*TODO: move*)
+(*TODO: when we add functions, this will become more complicated*)
+(*NOTE: this does NOT handle nested types (ex: tree = node of list tree)*)
+Definition is_ind_occ (ind: string) (t: ty) : bool :=
+  match t with
+  | ty_app ts tys => string_dec ind (ts_name ts)
+  | _ => false
+  end.
+
+(*Get all declared ADT names in a mutual block*)
+Definition mut_names (m: mut) : list string :=
+  map a_name (m_adts m).
+
+(*Filter out the recursive instances*)
+Definition get_nonind_vtys (l: list ty) : list ty :=
+  filter (fun v =>
+    forallb (fun ind => is_ind_occ ind v) (mut_names m)) l.
+
+(*Iterated tuple*)
+Fixpoint big_sprod (l: list Set) : Set :=
+  match l with
+  | nil => unit
+  | [x] => x
+  | x :: xs => (x * (big_sprod xs))%type
+  end.
+
+(*The type for a single constructor*)
+Definition build_constr_base (vars: list Set) (c: constr) : Set :=
+  big_sprod (map (ty_to_set vars) (get_nonind_vtys (c_args c))).
+
+Definition build_base (vars: list Set) (cs: list constr) : Set :=
+  in_type_extra _ constr_eq_dec cs (build_constr_base vars).
+
+End ADef.
+
+End Encode.
+
+End ADT.
